Spacetalk/HList.lean
@@ -19,21 +19,26 @@ inductive Member {α : Type u} : α → List α → Type u
   | head : Member a (a::as)
   | tail : Member a bs → Member a (b::bs)
 
+@[simp]
 def Member.toIndex : Member a as → Nat
   | head => 0
   | tail m => 1 + m.toIndex
 
+@[simp]
 def Member.compare (m1 : Member a as) (m2 : Member b bs) : Bool :=
   m1.toIndex == m2.toIndex
 
+@[simp]
 def Member.beq : Member a as → Member a as → Bool
   | .head, .head => true
   | .tail x, .tail y => Member.beq x y
   | _, _ => false
 
+@[simp]
 instance : BEq (Member a as) where
   beq := Member.beq
 
+@[simp]
 def Member.decEq : (x : Member a as) → (y : Member a as) → Decidable (x = y)
   | .head, .head => isTrue rfl
   | .tail x, .tail y =>
@@ -73,26 +78,31 @@ theorem Member.to_mem : Member a l → a ∈ l
   | .head => List.mem_of_mem_head? rfl
   | .tail i => List.mem_of_mem_tail i.to_mem
 
+@[simp]
 def Member.append_left {l₁ : List α} {l₂ : List α} : Member a l₁ → Member a (l₁ ++ l₂)
   | .head => .head
   | .tail i' => .tail i'.append_left
 
+@[simp]
 def Member.append_right {l₁ : List α} {l₂ : List α} (ia : Member a l₂) : Member a (l₁ ++ l₂) :=
   match l₁ with
   | [] => ia
   | _::_ => .tail ia.append_right
 
+@[simp]
 def List.replaceMember {α : Type u} {a : α} : (l : List α) → Member a l → α → List α
   | [], _, _ => []
   | _::t, .head, x => x :: t
   | h::t, .tail m, x => h :: t.replaceMember m x
 
+@[simp]
 def List.nthMember : (l : List α) → (n : Fin l.length) → Member (l.get n) l
   | _::_, ⟨0, _⟩ => .head
   | _::t, ⟨n'+1, _⟩ => .tail (t.nthMember ⟨n', _⟩)
 
 namespace HList
 
+  @[simp]
   def length : HList β is → Nat := λ_ ↦ is.length
 
   @[simp]
@@ -100,26 +110,32 @@ namespace HList
     | a ::ₕ as, .head => a
     | _ ::ₕ as, .tail h => as.get h
 
+  @[simp]
   def getNth : (l : HList β is) → (n : Fin is.length) → β (is.get n)
     | h ::ₕ _, ⟨0, _⟩ => h
     | _ ::ₕ t, ⟨n + 1, _⟩ => t.getNth ⟨n, _⟩
 
+  @[simp]
   def append (hl₁ : HList β is1) (hl₂ : HList β is2) : HList β (is1 ++ is2) :=
     match hl₁, hl₂ with
     | []ₕ, l => l
     | (h ::ₕ s), t => h ::ₕ s.append t
 
+  @[simp]
   def replace : HList β is → Member i is → β i → HList β is
     | []ₕ, _, _ => []ₕ
     | _::ₕt, .head, x => x ::ₕ t
     | h::ₕt, .tail m, x => h ::ₕ t.replace m x
 
+  @[simp]
   def head : HList β (i::is) → β i
     | h ::ₕ _ => h
 
+  @[simp]
   def tail : HList β (i::is) → HList β is
     | _ ::ₕ t => t
 
+  @[simp]
   def split {α : Type v} {β : α → Type u} {is1 is2 : List α} (hl : HList β (is1 ++ is2)) : HList β is1 × HList β is2 :=
     match is1 with
       | [] => ([]ₕ, hl)
@@ -137,6 +153,7 @@ infixr:67 " ++ₕ " => HList.append
 -- Given a List α, a function f : α → β,
 -- return a HList with indices of type β and values of β-indexed type δ
 -- using the mapping function g : (a : α) → δ (f a).
+@[simp]
 def List.toHList {α : Type v1} {β : Type v2} {δ : β → Type u}
                   (f : α → β) (g : (a : α) → δ (f a))
                   : (l : List α) → HList δ (l.map f)
