Spacetalk/Scratch.lean
@@ -1,0 +1,64 @@
+
+-- inductive Ty
+--   | bool
+--   | nat
+-- deriving DecidableEq
+
+-- def Ty.denote : Ty → Type
+--   | bool => Bool
+--   | nat => Nat
+
+-- inductive Typ
+--   | bool
+--   | nat
+-- deriving DecidableEq
+
+-- def Typ.denote : Typ → Type
+--   | bool => Bool
+--   | nat => Nat
+
+-- def Ty.toTyp : Ty → Typ
+--   | bool => .bool
+--   | nat => .nat
+
+-- import Mathlib.Data.List.Basic
+
+-- structure Foo where
+--   l : List Nat
+
+-- structure Bar (l : List Nat) where
+--   n : Nat
+--   mem : n ∈ l
+
+-- def find (foo : Foo) (n : Nat) : Option (Bar foo.l) :=
+--   match h : foo.l.find? (· = n) with
+--   | some x =>
+--     some ⟨n, by
+--       have hmem := List.mem_of_find?_eq_some h
+--       have heq := List.find?_some h
+--       simp_all
+--     ⟩
+--   | none => none
+
+-- example : find ⟨[0]⟩ 0 = some ⟨0, by simp⟩ := by
+--   simp [find]
+--   have heq : List.find? (· = 0) [0] = some 0 := by simp
+--   rw [heq]
+
+inductive Ty
+  | bv : Nat → Ty
+
+@[reducible]
+def Ty.denote : Ty → Type
+  | bv w => BitVec w
+
+inductive BinOp : Ty → Ty → Ty → Type
+  | add : {w : Nat} → BinOp (.bv w) (.bv w) (.bv w)
+  | eq : BinOp α α (.bv 1)
+
+def BinOp.eval : BinOp α β γ → (α.denote → β.denote → γ.denote)
+  | add => BitVec.add
+  | eq => λ a b => if a == b then ⟨1⟩ else ⟨0⟩
+
+example : ∀α x y (op : BinOp α α α), op.eval x y = op.eval x y := by
+  simp
